theories/Testing_Pre_orders/Must/Alternative_Preorder/Co_Inductive_Acceptance_Set/Equivalence/SoundnessCI.v
@@ -58,74 +58,79 @@ Proof.
     eapply convergence_set_if_convergence_forall in hcnv.
     constructor. eapply c_cnv. eapply equiv_termination. exact hcnv.
   + eapply convergence_forall_if_convergence_set. constructor.
-    - eapply c_cnv. admit.
-    - intros. eapply IHs.
-    co_preserved_by_wt_nil;eauto. eassumption.
-  eapply termination_if_termination_set_helper. constructor.
-  
-   intros. assert (q ⤓) by (now eapply c_cnv; intros; destruct (hcnv p H2)).
-    assert (hcnv0 : ∀ p : P, p ∈ ps → p ⇓ [a]).
-    intros p' mem'%hcnv.
-    constructor. now destruct mem'.
-    intros p1 hw1. inversion mem'; subst. eapply H7 in hw1. inversion hw1; subst.
-    now constructor.
-    now constructor.
-    eapply cnv_act; eauto.
-    intros q' hw.
-    eapply wt_decomp_one in hw as (q0' & q1' & q1 & hlt & hw0').
-    assert (hpre : ps ⩽ q). constructor; eauto.
-    eapply IHs; eauto.
-    ++ eapply co_preserved_by_wt_nil. eassumption.
-       eapply (co_preserved_by_wt_nil ps q q0') in hpre. destruct hpre.
-       eapply (c_step0 a q1'); eauto.
-       eapply (wt_s_set_from_pset_ispec ps [a] hcnv0); eauto. eassumption.
-    ++ intros p mem.
-       edestruct (wt_s_set_from_pset_ispec ps [a] hcnv0).
-       eapply H3 in mem as (p0 & hmem0%hcnv & hw0).
-       inversion hmem0; subst. eauto.
+    - eapply c_cnv. eapply convergence_set_iff_convergence_forall in hcnv.
+      inversion hcnv; eauto.
+    - intros. assert (∀ p : P, p ∈ ps → p ⇓ [a]) as hcnv_a.
+      { eapply convergence_forall_if_convergence_set.
+        eapply convergence_set_if_convergence_forall in hcnv. eapply cnv_wk;eauto. }
+      eapply convergence_set_if_convergence_forall.
+      eapply (IHs (wt_s_set_from_pset ps [a] hcnv_a));eauto.
+      * eapply c_step.
+        ++ eapply convergence_set_if_convergence_forall in hcnv_a. exact hcnv_a.
+        ++ intros q' mem'. eapply wk_tr_inv in H0 as (q'' & wk_tr'' & mem'');eauto.
+        ++ exact (wt_s_set_from_pset_ispec ps [a] hcnv_a).
+      * intros. edestruct (wt_s_set_from_pset_ispec ps [a] hcnv_a) as (Hyp1 & Hyp2).
+        eapply Hyp1 in H1 as (p' & mem & wk_tr). eapply hcnv in mem.
+        eapply cnv_preserved_by_wt_act;eauto.
 Qed.
 
-Lemma prex2_if_copre
-  `{@FiniteImagegLts P A H gLtsP, @FiniteImagegLts Q A H gLtsQ}
-  `{PreAP : @PreExtAction P A H FinA PreA PreA_eq PreA_countable 𝝳 Φ gLtsP}
-  `{PreAQ : @PreExtAction Q A H FinA PreA PreA_eq PreA_countable 𝝳 Φ gLtsQ}
-  (ps : gset P) (q : Q) : ps ⩽ q -> ps ₂≼ₛₑₜ_ₐₛ q.
+Lemma prex2_if_copre `{
+  gLtsP : @gLts P A H, !FiniteImagegLts P A, AbsPT : @AbsAction P T FinA PreAct A H Φ 𝝳P  gLtsP gLtsT,
+  gLtsQ : @gLts Q A H, !FiniteImagegLts Q A, AbsQT : @AbsAction Q T FinA PreAct A H Φ 𝝳Q  gLtsQ gLtsT}
+  (ps : gset P) (qs : gset Q) : ps ⩽ qs -> ps ₂≼ₛₑₜ_ₐₛ qs.
 Proof.
-  revert ps q.
-  intros ps q hsub s.
-  revert ps q hsub.
-  dependent induction s; intros ps q hsub.
-  + intros q' hw hstq' hcnv.
-    dependent induction hw; try rename p into q.
-    ++ destruct hsub.
-       edestruct c_now.
-       intros p0 mem0. edestruct (hcnv p0 mem0); eauto. eassumption.
-       decompose record H2. repeat eexists;  eauto.
-    ++ eapply IHhw; eauto. destruct hsub. eapply c_tau. eassumption.
+  revert ps qs.
+  intros ps qs hsub q s.
+  revert ps qs q hsub.
+  dependent induction s; intros ps qs q hsub.
+  + intros q' mem hw hstq' hcnv. revert ps qs hstq' hcnv mem hsub.
+    dependent induction hw; try rename p into q; intros.
+    ++ destruct hsub. edestruct c_now;eauto.
+       - eapply equiv_termination. eapply convergence_set_if_convergence_forall; eauto.
+    ++ eapply IHhw.
+       - eauto.
+       - eauto.
+       - eauto.
+       - eapply elem_of_singleton. reflexivity.
+       - eapply c_tau. eassumption.
+         intros q' mem'. assert (q' = q) by set_solver. subst.
+         exists p. split; eauto. eapply lts_to_wt_tau;eauto.
   + intros. rename a into μ.
-    replace (μ :: s) with ([μ] ++ s) in H2 by eauto.
-    eapply wt_split in H2 as (q0 & hw0 & hw1).
+    replace (μ :: s) with ([μ] ++ s) in H1 by eauto.
+    eapply wt_split in H1 as (q0 & hw0 & hw1).
     eapply wt_decomp_one in hw0 as (q0' & q1' & q1 & hlt & hw0').
-    assert (ps ⩽ q0') by (eapply co_preserved_by_wt_nil; eauto).
+    assert (ps ⩽ {[q0']}).
+    { eapply co_preserved_by_wt_nil; eauto. intros q'' mem''.
+      assert (q0' = q'') by set_solver. subst. exists q. split;eauto. }
     assert (hcnv' : ∀ p : P, p ∈ ps → p ⇓ [μ]).
-    intros. constructor. edestruct (H4 p H5); eauto.
-    intros. constructor. eapply cnv_terminate.
-    eapply cnv_preserved_by_wt_act; eauto.
+    { intros. constructor. edestruct (H3 p H4); eauto.
+      intros. constructor. eapply cnv_terminate.
+      eapply cnv_preserved_by_wt_act; eauto. }
     set (ps' := wt_s_set_from_pset ps [μ] hcnv').
-    assert (ps ⩽ q0') by (eapply co_preserved_by_wt_nil; eauto).
-    assert (ps' ⩽ q1'). destruct H2.
-    eapply c_step. eassumption. eassumption.
-    eapply wt_s_set_from_pset_ispec.
-    assert (ps' ⩽ q0) by (eapply co_preserved_by_wt_nil; eauto).
-    edestruct (IHs ps' q0 H7 _ hw1 H3) 
+    assert (ps ⩽ {[ q0' ]}).
+    { eapply co_preserved_by_wt_nil; eauto. intros q'' mem''.
+      assert (q0' = q'') by set_solver. subst. exists q''. split;eauto. eapply wt_nil. }
+    assert (ps' ⩽ {[ q1' ]}). 
+    { destruct H4. eapply c_step.
+      + eapply convergence_set_if_convergence_forall. exact hcnv'.
+      + intros q''' mem'''.
+        assert(q''' = q1') by set_solver. subst.
+        exists q0'. split. set_solver. eapply lts_to_wt. exact hlt.
+      + eapply wt_s_set_from_pset_ispec. }
+    assert (ps' ⩽ {[ q0 ]}).
+    { eapply co_preserved_by_wt_nil; eauto.
+      intros q'' mem''. exists q1'. split. set_solver.
+      assert (q'' = q0) by set_solver. subst. eauto. }
+    assert (q0 ∈ ({[q0]}: gset Q)) as mem_sing by set_solver.
+    edestruct (IHs ps' ({[ q0 ]}) q0 H6 _ mem_sing hw1 H2) 
     as (r & memr & p' & hwr & hst & hsub').
-    intros.
-    edestruct (wt_s_set_from_pset_ispec ps [μ] hcnv').
-    eapply H9 in H8 as (p0  & hmem0 & hw0).
-    eapply cnv_preserved_by_wt_act; eauto.
-    edestruct (wt_s_set_from_pset_ispec ps [μ] hcnv').
-    eapply H8 in memr as (p0  & hmem0 & hw0).
-    exists p0. split. eassumption. exists p'. split.
-    eapply wt_push_left; eassumption.
-    split; eauto.
+    * intros. edestruct (wt_s_set_from_pset_ispec ps [μ] hcnv') as (Hyp1 & Hyp2). 
+      eapply Hyp1 in H7 as (p0  & hmem0 & hw0).
+      eapply cnv_preserved_by_wt_act; eauto.
+    * edestruct (wt_s_set_from_pset_ispec ps [μ] hcnv') as (Hyp1 & Hyp2).
+      eapply Hyp1 in memr as (p0  & hmem0 & hw0).
+      exists p0. split ;eauto. exists p'.
+      split.
+      ++ eapply wt_push_left; eassumption.
+      ++ split;eauto.
 Qed.
